Splinter/Paged/LinkedJournal.i.dfy
@@ -1,26 +1,41 @@
+// Copyright 2018-2021 VMware, Inc., Microsoft Inc., Carnegie Mellon University, ETH Zurich, and University of Washington
+// SPDX-License-Identifier: BSD-2-Clause
 
+include "PagedJournal.i.dfy"
+
+// The plan is something that refines to a TruncatedJournal.
 
 module LinkedJournal {
-  type Pointer = nat
+  import opened Options
+  import opened MsgHistoryMod
+  import opened LSNMod
+
+  import PagedJournalIfc = PagedJournal // TODO(jonh): crack out ifc
+
+  type Pointer(==,!new)
+
+  datatype CacheView = CacheView(entries: map<Pointer, JournalRecord>) {
+    function I(opointer: Option<Pointer>, used: set<Pointer>) : Option<PagedJournalIfc.JournalRecord>
+      decreases entries.Keys - used
+    {
+      if opointer.None?
+      then None
+      else
+      var pointer := opointer.value;
+      if pointer in used
+      then None // Pointer cycle; fail.
+      else if pointer !in entries
+      then None
+      else
+        var entry := entries[pointer];
+        Some(PagedJournalIfc.JournalRecord(entry.messageSeq, I(entry.priorRec, used + {pointer})))
+    }
+  }
 
   datatype JournalRecord = JournalRecord(
     messageSeq: MsgHistory,
     priorRec: Option<Pointer>
   )
-  {
-    function I(cacheView: CacheView) : PagedJournalIfc.JournalRecord
-    {
-      PagedJournalIfc.JournalRecord(messageSeq,
-        if priorRec.None?
-        then None
-        else if priorRec.value !in cacheView
-        then None
-        else Some(cacheView[priorRec.value].I(cacheView))
-      )
-    }
-  }
-
-  type CacheView = map<Pointer, JournalRecord>
 
   datatype TruncatedJournal = TruncatedJournal(
     boundaryLSN : LSN,  // exclusive: lsns <= boundaryLSN are discarded
@@ -29,9 +44,13 @@ module LinkedJournal {
   {
     function I() : PagedJournalIfc.TruncatedJournal
     {
-  
+      PagedJournalIfc.TruncatedJournal(boundaryLSN, cacheView.I(freshestRec, {}))
     }
   }
 
-
+  // implementation of JournalIfc obligations
+  function Mkfs() : (out:PersistentJournal)
+  {
+    TruncatedJournal(0, None)
+  }
 }
