Splinter/Paged/StampedMap.i.dfy
@@ -5,6 +5,7 @@ include "../../lib/Lang/NativeTypes.s.dfy"
 include "../../lib/Base/KeyType.s.dfy"
 include "../../Spec/Message.s.dfy"
 include "../../Spec/TotalKMMap.s.dfy"
+include "LSNMod.i.dfy"
 
 // A "StampedMap" is a full imap "stamped" with an LSN that identifies how many
 // operations it represents.
@@ -12,8 +13,7 @@ module StampedMapMod {
   import opened ValueMessage
   import opened KeyType
   import opened TotalKMMapMod
-
-  type LSN = nat // Log sequence number
+  import opened LSNMod
 
   datatype StampedMap = StampedMap(mi: TotalKMMap, seqEnd: LSN)
 
